sanity check: the new wp-pweq rule would indeed help for Report Noisy Max

theories/diffpriv_simple_pw/examples/report_noisy_max.v
@@ -26,29 +26,6 @@ Section rnm.
               "rnm" ("i" + #1)))
       in "f" #0.
 
-  (* Really, the guard on the if statement that ensures initialization on the
-     first iteration should be pulled out of the recursion as follows:
-
-  Definition report_noisy_max (num den : Z) : val :=
-    λ:"evalQ" "N" "d",
-      if: "N" ≤ #0 then #(-1) else
-      let: "maxI" := ref #0 in
-      let: "maxA" := ref #0 in
-      let: "f" :=
-        (rec: "rnm" "i" :=
-           if: "i" = "N" then
-             ! "maxI"
-           else
-             (let: "a" := Laplace #num #(2*den) ("evalQ" "i" "d") in
-              (if: ! "maxA" < "a" then
-                 "maxA" <- "a" ;;
-                 "maxI" <- "i"
-               else #()) ;;
-              "rnm" ("i" + #1)))
-      in "f" #0.
-
- *)
-
   Definition rnm_body (num den : Z) (evalQ : val) {DB} (dDB : Distance DB) (N : nat) (db : DB) (maxI maxA : loc) :=
     (rec: "rnm" "i" :=
        if: "i" = #N then ! #maxI
@@ -56,141 +33,6 @@ Section rnm.
             (if:  "i" = #0 `or` ! #maxA < "a"
              then #maxA <- "a";; #maxI <- "i" else #());;
             "rnm" ("i" + #1))%V.
-
-  (* An online version of RNM (oRNM) providing two methods:
-- add_query receives and evaluates queries one at a time, storing the highest (noisy) result,
-- release outputs the index of the query with the highest result. *)
-  Definition report_noisy_max_online : val :=
-    λ:"num" "den" "evalQ" "d",
-      let: "maxI" := ref #(-1) in
-      let: "maxA" := ref #0 in
-      let: "add_query" :=
-        λ:"i",
-          (let: "a" := Laplace "num" (#2 * "den") ("evalQ" "i" "d") in
-           (if: "i" = #0 `or` ! "maxA" < "a" then
-              "maxA" <- "a" ;;
-              "maxI" <- "i"
-            else #())) in
-      let: "release" :=
-        λ:"_",
-          ! "maxI"
-      in ("add_query", "release").
-
-  (* Given the error credits for one run of RNM, initializing oRNM provides an abstract token AUTH
-  that is required to call the add_query and release methods, and...
-- add_query processes a query and returns AUTH back to the caller
-- release consumes the AUTH token and ensures that both db and db' yield (pointwise) equal results *)
-  Lemma rnm_online (j : Z) (num den : Z) (evalQ : val)
-    (εpos : 0 < IZR num / IZR den) `(dDB : Distance DB) (db db' : DB) (adj : dDB db db' <= 1) K
-    :
-    (∀ i, wp_sensitive (Val evalQ i) 1 dDB dZ) -∗
-    ↯m (IZR num / IZR den) -∗
-
-    ⤇ fill K (report_noisy_max_online #num #den (Val evalQ) (inject db')) -∗
-    WP report_noisy_max_online #num #den evalQ (inject db)
-
-      {{ add_release,
-           ∃ (add' release' : val) (AUTH : iProp Σ),
-
-             ⤇ fill K (add', release')%V ∗
-
-             AUTH ∗
-
-             (∀ K i,
-                 AUTH -∗
-                 ⤇ fill K (add' #i) -∗
-                 WP (Fst (Val add_release) #i) {{ _, ⤇ fill K #() ∗ AUTH }}) ∗
-
-             (∀ K,
-                 AUTH -∗
-                 ⤇ fill K (release' #()) -∗
-                 WP (Snd (Val add_release) #())
-                   {{ v, ∃ v' : val, ⌜ v = #j → v' = #j ⌝ }})
-            }}.
-  Proof with (tp_pures ; wp_pures).
-    (* The privacy proof of RNM hinges on the fact that the credit gets spent when the "winning"
-    query gets evaluated, i.e., when the index matches that of the result in the point-wise
-    equality.
-
-    For oRNM, the result index in the point-wise equality of the release method can either be
-    quantified before or after the initialisation of oRNM. Knowing the index is required to decide
-    which coupling to spend the credit on. If the index is quantified in the spec for `release`,
-    then `add` cannot know about it, and we don't know how to couple.
-
-    This is why this current spec quantifies over `i : Z` before initialising oRNM. *)
-
-    (* NB: Actually, since we require to know `j` in advance, we could also make the queries on
-    `i≠j` free and only require ↯ε on the j-th query. *)
-
-    iIntros "sens ε rhs".
-    rewrite /report_noisy_max_online... simpl...
-    tp_alloc as maxI2 "maxI2". tp_pures. tp_alloc as maxA2 "maxA2". do 5 tp_pure.
-    wp_pures. wp_alloc maxI1 as "maxI1". wp_alloc maxA1 as "maxA1". do 5 wp_pure.
-    simpl...
-    iExists _,_.
-    (* TODO: This is too simple-minded; the availability of ε in AUTH has to depend on whether or
-    not `i` has been queried. *)
-    iExists (
-        maxI2 ↦ₛ #(-1) ∗
-        maxA2 ↦ₛ #0 ∗
-        maxI1 ↦ #(-1) ∗
-        maxA1 ↦ #0 ∗
-        ↯m (IZR num / IZR den)
-      )%I.
-    iFrame.
-    clear K.
-    iModIntro. iSplitL.
-    - iIntros "%K %i (maxI2 & maxA2 & maxI1 & maxA1 & ε) rhs".
-      admit.
-    - iIntros "%K (maxI2 & maxA2 & maxI1 & maxA1 & ε) rhs".
-      admit.
-  Abort.
-
-  (* The above-mentioned issue with anticipating when an error-credit gets spent by examining the
-  index returned as final result can be exhibited in an example simpler than oRNM.
-
-   This problem can be stated in Eris as follows. Sufficient use of laziness in `get` might solve
-   this particular problem. *)
-
-  Goal
-    ↯m (1/4)  -∗
-    WP
-      let: "res" := ref (rand #3) in
-      let: "resample" := λ:"_", "res" <- rand #3 in
-      let: "get" := λ:"_", !"res" in
-      ("resample", "get")
-        {{ resample_get ,
-             let (resample, get) := ((Fst (Val resample_get))%E, (Snd (Val resample_get))%E) in
-             ∃ TOKEN : iProp Σ,
-               TOKEN ∗
-               (TOKEN -∗ WP resample #() {{ _, TOKEN }}) ∗
-               (TOKEN -∗ WP get #() {{ v, ∃ k : Z, ⌜v = #k⌝ ∗ ⌜0 < k⌝%Z }})
-        }}.
-  Abort.
-
-  (* One can generalize this argument by parametrising `resample` by some function `f` which is
-  (i) known to be safe, and (ii) produces the result 1 if given some resource `X`.
-
-    This is now a problem in unary separation logic, although it is not immediate what `X` and `f` should be.
-   *)
-  Goal
-    ∀ (f : val), ∃ (X : iProp Σ),
-      (X -∗ WP (Val f) #()  {{ v, ⌜v = #1⌝}}) -∗
-      (WP (Val f) #()  {{ _, ⌜True⌝ }}) -∗
-      X -∗
-      WP
-        let: "res" := ref (f #()) in
-        let: "resample" := (λ:"_", "res" <- f #()) in
-        let: "get" := (λ:"_", !"res") in
-        ("resample", "get")
-          {{ resample_get ,
-               let (resample, get) := ((Fst (Val resample_get))%E, (Snd (Val resample_get))%E) in
-               ∃ TOKEN,
-                 TOKEN ∗
-                 (TOKEN -∗ WP resample #() {{ _, TOKEN }}) ∗
-                 (TOKEN -∗ WP get #() {{ v, ∃ k : Z, ⌜v = #k⌝ ∗ ⌜0 < k⌝%Z }})
-          }}.
-  Abort.
 
   (* This proof is *almost* completed modulo the (impossible) case where the return value `j` is
      not a positive integer. *)
@@ -586,138 +428,44 @@ Section rnm.
   (* Qed. *)
   Admitted.
 
-  Definition WP_PWEQ := ∀ e e' K E,
-    (
-      ⤇ fill K e' ⊢
-      ∀ (RES : val),
-          WP e @ E
-            {{ v, ∃ v' : val, ⤇ fill K (Val v') ∗ ⌜v = RES → v' = RES⌝ }} )
-→
-    (⤇ fill K e'
-    ⊢
-     WP e @ E
-      {{ v, ∃ v' : val, ⤇ fill K (Val v') ∗ ⌜v = v'⌝ }}).
 
-
-  (* unclear how to close because the error resources don't work out *)
-  (* Lemma rnm_diffpriv num den (evalQ : val) DB (dDB : Distance DB) (N : nat) K :
-       (0 < IZR num / IZR (2 * den)) →
-       (∀ i : Z, ⊢ hoare_sensitive (evalQ #i) 1 dDB dZ) →
-       ∀ db db', dDB db db' <= 1 →
-                 WP_PWEQ →
-                   ↯m (IZR num / IZR den) ∗
-                       ⤇ fill K (report_noisy_max num den evalQ #N (inject db'))
-                       ⊢
-                         WP report_noisy_max num den evalQ #N (inject db)
-                           {{ v, ∃ (v' : val), ⤇ fill K v' ∗ ⌜ v = v' ⌝  }}
-     .
-     Proof.
-       intros ????? wp_pweq. iIntros "(ε & rhs)".
-       iPoseProof (wp_pweq with "[$rhs]") as "pweq".
-       iApply (wp_pweq with "[$rhs]") ; iIntros "rhs %RES".
-       iApply (rnm_pw_diffpriv with "[$ε $rhs]") => //.
-       by iNext ; iIntros.
-     Qed. *)
-
-  Lemma wp_pweq_couple : WP_PWEQ.
+  Lemma rnm_diffpriv num den (evalQ : val) DB (dDB : Distance DB) (N : nat) K :
+    (0 < IZR num / IZR (2 * den)) →
+    (∀ i : Z, ⊢ hoare_sensitive (evalQ #i) 1 dDB dZ) →
+    ∀ db db', dDB db db' <= 1 →
+                ↯m (IZR num / IZR den) ∗
+                    ⤇ fill K (report_noisy_max num den evalQ #N (inject db'))
+                    ⊢
+                      WP report_noisy_max num den evalQ #N (inject db)
+                        {{ v, ∃ (v' : val), ⤇ fill K v' ∗ ⌜ v = v' ⌝  }}
+  .
   Proof.
-    iLöb as "IH". iIntros (e e' K E).
-    iIntros "%pw rhs".
-    (* iIntros "[rhs pw] /=". *)
-    rewrite wp_unfold /wp_pre //=.
-    setoid_rewrite wp_unfold at 3.
-    rewrite {1}/wp_pre /=.
-    iIntros (?????) "([H T] & S & ε & δ)".
-    iSpecialize ("pw" with "rhs").
-    destruct (to_val e) eqn:ev.
-    -
-      iSpecialize ("pw" $! v).
-      iMod ("pw" with "[$]") as "pw". iModIntro.
-      iApply (spec_coupl_mono ∅ with "[] pw") => //=.
-      iIntros (?????) "> (HT & S & E & %v' & rhs & %pweq)". iFrame.
-      rewrite pweq => //.
-    -
-      iApply spec_coupl_ret.
-      iSpecialize ("pw" with "[$H $T $S $ε $δ]").
-
-      fail.
-
-      iApply (prog_coupl_mono with "[pw] ") => //=.
-
-
-    (*   iApply fupd_mask_intro => //.
-         iIntros "hclose".
-       iApply spec_coupl_ret. iFrame.
-
-       rewrite spec_coupl_unfold /spec_coupl_pre //=.
-       iLeft.
-
-       rewrite wp_unfold /wp_pre //=.
-       rewrite ev.
-       iSpecialize ("pw" $! _ _ _ _ _).
-       iSpecialize ("pw" with "[$H $T $S $ε $δ]").
-         iFrame. iMod "hclose". iModIntro.
-         admit.
-       - *)
-  Admitted.
-
-
-  Corollary wp_pweq_couple_swap K (* E  *)e e' :
-    ⤇ fill K e' ∗
-    (∀ (RES : val),
-        ⤇ fill K e' -∗
-          WP e (* @ E *)
-            {{ v, ∃ v' : val, ⤇ fill K (Val v') ∗ ⌜v = RES → v' = RES⌝ }} )
-    -∗
-     WP e (* @ E *)
-      {{ v, ∃ v' : val, ⤇ fill K (Val v') ∗ ⌜v = v'⌝ }}.
-  Proof.
-    iIntros "[rhs pw]". iPoseProof (wp_pweq_couple e e' K with "[$rhs pw]") as "h".
-    2: iApply "h".
-    iIntros. iApply "pw". done.
+    intros ?????. iIntros "(ε & rhs)".
+    iApply (wp_pweq with "[ε] rhs") ; iIntros "%RES rhs".
+    iApply (rnm_pw_diffpriv with "[$ε $rhs]") => //.
+    iIntros "!> **". iFrame.
   Qed.
 
-
-  (* Lemma hoare_pweq_couple K E e e' ε :
-       {{{ ⤇ fill K e' ∗ ↯m ε ∗
-           (∀ (RES : val),
-               {{{ ⤇ fill K e' ∗ ↯m ε }}}
-                 e @ E
-                 {{{ (v : val), RET v; ∃ v' : val, ⤇ fill K (Val v') ∗ ⌜v = RES → v' = RES⌝ }}} )
-       }}}
-         e @ E
-         {{{ (v : val), RET v; ∃ v' : val, ⤇ fill K (Val v') ∗ ⌜v = v'⌝ }}}.
-     Proof.
-       iIntros (Φ) "[rhs [ε pw]] HΦ".
-       iPoseProof (wp_pweq_couple_swap with "[$rhs pw ε HΦ]") as "wppw" => //.
-       { iIntros "%RES rhs". iSpecialize ("pw" $! RES with "[$]").
-     Admitted.
-
-     (* persistence is annoying *)
-     Lemma hoare_pweq_couple' K E e e' num den :
-       {{{ ⤇ fill K e' ∗ ↯m (IZR num / IZR den) ∗
-           (∀ (RES : val),
-               {{{ ⤇ fill K e' ∗ ↯m (IZR num / IZR den) }}}
-                 e @ E
-                 {{{ (v : val), RET v; ∃ v' : val, ⤇ fill K (Val v') ∗ ⌜v = RES → v' = RES⌝ }}} )
-       }}}
-         e @ E
-         {{{ (v : val), RET v; ∃ v' : val, ⤇ fill K (Val v') ∗ ⌜v = v'⌝ }}}.
-     Proof.
-       (* iIntros "%φ [rhs [ε h]] hφ".
-          iApply (pweq_couple with "[$rhs h ε]") => //.
-          iIntros.
-          iIntros (ψ).
-          iSpecialize ("h" $! RES _).
-          iApply (wp_strong_mono'' with "h").
-          iApply "h".
-          iRevert "ε". *)
-     Admitted. *)
-
-
-
-
 End rnm.
+
+Lemma rnm_diffpriv_cpl_direct num den (evalQ : val) DB (dDB : Distance DB) (N : nat) :
+  (0 < IZR num / IZR (2 * den))%R →
+  (0 <= IZR num / IZR den)%R →
+  (∀ `{!diffprivGS Σ}, ∀ i : Z, ⊢ hoare_sensitive (evalQ #i) 1 dDB dZ) →
+  ∀ db db',
+    (dDB db db' <= 1)%R →
+    ∀ σ,
+      DPcoupl
+        (lim_exec ((report_noisy_max num den evalQ #N (inject db)), σ))
+        (lim_exec ((report_noisy_max num den evalQ #N (inject db')), σ))
+        (λ v v', v = v')
+        (IZR num / IZR den) 0
+.
+Proof.
+  intros. eapply (adequacy_simple_pw.wp_adequacy diffprivΣ) => //.
+  iIntros "% rnm' ε δ".
+  iApply (rnm_diffpriv _ _ _ _ _ N [] with "[$]") => //.
+Qed.
 
 
 Lemma rnm_pw_diffpriv_cpl num den (evalQ : val) DB (dDB : Distance DB) (N : nat) :
@@ -736,7 +484,7 @@ Lemma rnm_pw_diffpriv_cpl num den (evalQ : val) DB (dDB : Distance DB) (N : nat)
 .
 Proof.
   intros.
-  eapply (adequacy.wp_adequacy diffprivΣ) => //.
+  eapply (adequacy_simple_pw.wp_adequacy diffprivΣ) => //.
   iIntros (?) "rnm' ε".
   iPoseProof (rnm_pw_diffpriv num den evalQ DB dDB N [] H (H1 _ _) db db' H2 #j
     %I) as "h" => //.
@@ -768,7 +516,7 @@ Proof.
   apply DPcoupl_pweq => //. 1: apply ex_seriesC_0.
   simpl.
   intros x'.
-  eapply (adequacy.wp_adequacy diffprivΣ) => //.
+  eapply (adequacy_simple_pw.wp_adequacy diffprivΣ) => //.
   iIntros (?) "rnm' ε".
   unshelve iPoseProof (rnm_pw_diffpriv num den evalQ DB dDB N [] H (H1 _ _) db db' H2 x'
     (λ v, ∃ v' : val, ⤇ v' ∗ ⌜v = x' → v' = x'⌝)%I) as "h" => //.
@@ -780,7 +528,7 @@ Proof.
   apply h.
 Qed.
 
-Lemma rnm_diffpriv num den (evalQ : val) DB (dDB : Distance DB) (N : nat) :
+Lemma rnm_diffpriv' num den (evalQ : val) DB (dDB : Distance DB) (N : nat) :
   (0 < IZR num / IZR (2 * den))%R →
   (0 <= IZR num / IZR den)%R →
   (∀ `{!diffprivGS Σ}, ∀ i : Z, ⊢ hoare_sensitive (evalQ #i) 1 dDB dZ) →
@@ -794,124 +542,3 @@ Proof.
   intros. apply diffpriv_approx_pure. apply DPcoupl_diffpriv.
   intros. apply rnm_diffpriv_cpl => //.
 Qed.
-
-(* sketchy obsolete concrete example below *)
-
-(* Definition DB := (Z * Z * Z)%type. *)
-(* Definition dDB : Distance DB. *)
-(*   unshelve econstructor. *)
-(*   - exact (λ (x y : DB), match (x,y) with *)
-(*                          | ((x1, x2, x3), (y1, y2, y3)) => *)
-(*                              (if Z.eqb x1 y1 then 0 else 1) *)
-(*                              + (if Z.eqb x2 y2 then 0 else 1) *)
-(*                              + (if Z.eqb x3 y3 then 0 else 1) *)
-(*                          end). *)
-(*   - apply _. *)
-(*   - intros [[x1 x2] x3] [[y1 y2] y3]. destruct (x1 =? y1)%Z, (x2 =? y2)%Z, (x3 =? y3)%Z. *)
-(*     all: compute ; lra. *)
-(*   - simpl. intros [[x1 x2] x3] [[y1 y2] y3] [[-> ->] ->]. rewrite !Z.eqb_refl. compute ; lra. *)
-(*   - simpl. intros [[x1 x2] x3] [[y1 y2] y3]. *)
-(*     destruct (x1 =? y1)%Z eqn:h1, (x2 =? y2)%Z eqn:h2, (x3 =? y3)%Z eqn:h3 ; try (compute ; intuition auto ; try lra). *)
-(*     + rewrite (Z.eqb_eq x1 y1) // in h1. *)
-(*     + rewrite (Z.eqb_eq x2 y2) // in h2. *)
-(*     + rewrite (Z.eqb_eq x3 y3) // in h3.  *)
-(* Defined. *)
-
-Definition ID := Fst.
-Definition age := Snd.
-(* Two example databases with three rows each containing a ID number and an age. *)
-Definition db : val := ( (#3, #12), (#1, #42), (#0, #57) ).
-Definition db' : val := ( (#3, #12), (#2, #24), (#0, #57) ).
-
-Definition under_40 : val := λ:"r", if: age "r" < #40 then #1 else #0.
-Definition over_80 : val := λ:"r", if: #80 < age "r" then #1 else #0.
-Definition setmap : val := λ: "f" "db", ("f" (Fst (Fst "db")) , "f" (Snd (Fst "db")) , "f" (Snd "db")).
-Definition setsum : val := λ: "db", (Fst (Fst "db")) + (Snd (Fst "db")) + (Snd "db").
-Definition count_query (num den : Z) : val := λ:"b", setsum (setmap (λ:"z", Laplace #num #den "z") (setmap under_40 "b")).
-
-Definition count_under_40 : val := λ:"db", setsum $ setmap under_40 "db".
-Definition count_over_80 : val := λ:"db", setsum $ setmap over_80 "db".
-
-Definition evalQ : val :=
-  λ:"i" "db", if: "i" = #0 then count_under_40 "db"
-              else if: "i" = #1 then count_over_80 "db"
-                   else #0.
-
-(* concrete example run *)
-(* Lemma rnm_diffpriv_3 num den :
-       (0 < IZR num / IZR den) →
-       ∀ (K : list (ectxi_language.ectx_item prob_ectxi_lang)),
-         {{{ ⤇ fill K (report_noisy_max num den evalQ #2 (inject db')) ∗
-             ↯m (IZR num / IZR den)
-               (* ↯m 0 *)
-         }}}
-           (report_noisy_max num den evalQ #2 (inject db))
-           {{{ (v : val), RET v; ⤇ fill K v }}}.
-     Proof.
-       iIntros (???) "[rnm' ε] hφ".
-       rewrite /report_noisy_max.
-       simpl.
-       tp_pures.
-       tp_alloc as maxI2 "maxI2". tp_pures. tp_alloc as maxA2 "maxA2". do 5 tp_pure.
-       wp_pures. wp_alloc maxI1 as "maxI1". wp_alloc maxA1 as "maxA1". do 5 wp_pure.
-       wp_rec. wp_pures.
-       tp_pures.
-       rewrite {2 4}/evalQ. tp_pures. wp_pures.
-       rewrite /count_under_40/setsum/setmap/under_40/age. wp_pures. tp_pures.
-
-       wp_bind (Laplace _ _ _). tp_bind (Laplace _ _ _).
-       iMod ecm_zero as "ε0".
-       unshelve iApply (hoare_couple_laplace 1 2 1 0 _ (num) (2*den) _ _  (AppRCtx _ :: K)
-           with "[ε0 $rnm']" ) => //=.
-       1: by cbv.
-       { rewrite mult_IZR.
-         rewrite Rmult_comm.
-         rewrite Rdiv_mult_distr.
-         rewrite {1}/Rdiv.
-         revert H.
-         set (r := (IZR num / IZR den)).
-         lra.
-       }
-       1: rewrite Rmult_0_l => //.
-       simpl. tp_pures.
-       iIntros "!> %z f'" => /=. wp_pures. tp_pures. tp_load ; wp_load. wp_pures.
-       wp_load. tp_pures. tp_load. tp_pures. wp_pures.
-       tp_store. tp_pures. tp_store. do 2 wp_store. wp_pures. tp_pures.
-       rewrite {2 4}/evalQ. tp_pures. 1,2: try naive_solver. wp_pures.
-       rewrite /count_over_80/setsum/setmap/over_80/age. wp_pures. tp_pures.
-       wp_bind (Laplace _ _ _). tp_bind (Laplace _ _ _).
-       iMod ecm_zero as "ε0".
-       unshelve iApply (hoare_couple_laplace _ _ 0 0 _ (num) (2*den) _ _  (AppRCtx _ :: K)
-           with "[ε ε0 $f']" ) => //=.
-       1: try naive_solver.
-       { rewrite mult_IZR.
-         rewrite Rmult_comm.
-         rewrite Rdiv_mult_distr.
-         rewrite {1}/Rdiv.
-         revert H.
-         set (r := (IZR num / IZR den)).
-         lra.
-       }
-       (* 1: rewrite Rmult_1_l => //. 1:admit. *)
-       1: rewrite Rmult_0_l => //.
-       simpl. tp_pures.
-       iIntros "!> %z2 f'" => /=. wp_pures. tp_pures. tp_load ; wp_load. wp_pures.
-       wp_load. wp_pures.
-       tp_pures. tp_load. tp_pures.
-       rewrite !Zplus_0_r ?Zplus_0_l.
-       case_bool_decide.
-       - do 2 wp_store. wp_pures.
-         tp_pures. tp_store ; tp_pures ; tp_store ; tp_pures.
-         tp_load.
-         wp_load.
-         iApply "hφ". done.
-         Unshelve.
-         2: f_equal. simpl.
-       - wp_pures.
-         tp_pures.
-         tp_load.
-         wp_load.
-         iApply "hφ". done.
-         Unshelve.
-         all: f_equal.
-     Qed. *)
